REALLY SLOW implementation based on rewriting.
- It does work but it is really slow.
- There are several potential ways to optimize this
  1) rewrite_strat
  2) computational reflection
  3) mtac

theories/OrderedTerms.v
@@ -5,7 +5,7 @@ Require Import Coq.Classes.Morphisms.
 Set Implicit Arguments.
 Set Strict Implicit.
 
-Record Order (T : Type) : Type :=
+Class Order (T : Type) : Type :=
 { le : T -> T -> Prop
 ; Refl_le :> Reflexive le
 ; Trans_le :> Transitive le }.
@@ -14,8 +14,16 @@ Arguments Refl_le {_ _} _.
 Arguments Trans_le {_ _} _ _ _ _ _.
 
 Record otype : Type :=
-{ T :> Type ; order :> Order T }.
+{ T :> Type
+; order :> Order T }.
 (* 'equality' is defined as 'a <= b /\ b <= a' *)
+
+Existing Instance order.
+
+Definition ole {T : otype} (a b : T) : Prop :=
+  le a b.
+Definition oequiv {T : otype} (a b : T) : Prop :=
+  ole a b /\ ole b a.
 
 (* The discrete ordering *)
 Definition otype_eq (T : Type) : otype.
@@ -25,21 +33,27 @@ eauto. eauto with typeclass_instances.
 Defined.
 
 
-Definition Order_pair (A B : Type) `{OA : Order A} `{OB : Order B} : Order (A * B).
+Definition Order_prod (A B : Type) `{OA : Order A} `{OB : Order B}
+: Order (A * B).
 refine
 {| le := fun a b => @le _ OA (fst a) (fst b) /\ @le _ OB(snd a) (snd b) |}.
 { split; apply Refl_le. }
 { red. destruct 1; destruct 1; split; eapply Trans_le; eassumption. }
 Defined.
 
-Canonical Structure otype_pair (a b : otype) : otype := (* canonical structure *)
-{| T := a.(T) * b.(T) ; order := @Order_pair a.(T) b.(T) a.(order) b.(order) |}.
+Canonical Structure otype_prod (a b : otype) : otype := (* canonical structure *)
+{| T := a.(T) * b.(T)
+; order := @Order_prod a.(T) b.(T) a.(order) b.(order) |}.
 
-Definition Order_fun (A B : Type) `{OA : Order A} `{OB : Order B}
-: Order { f : A -> B & Proper (@le _ OA ==> @le _ OB) f }.
+Record PFun (A B : otype) : Type :=
+{ function : A -> B
+; Proper_function : Proper (ole ==> ole) function }.
+
+Definition Order_fun (A B : otype)
+: Order (PFun A B).
 refine
-{| le := fun a b => (@le _ OA ==> @le _ OB)%signature (projT1 a) (projT1 b) |}.
-{ red. red. intros. destruct x. simpl. apply p. assumption. }
+{| le := fun a b => (ole ==> ole)%signature (function a) (function b) |}.
+{ red. red. intros. destruct x. simpl. apply Proper_function0. assumption. }
 { red. red. intros.
   eapply Trans_le.
   eapply H. eassumption.
@@ -47,8 +61,8 @@ refine
 Defined.
 
 Definition otype_fun (a b : otype) : otype :=
-{| T := { f : a.(T) -> b.(T) & Proper (le ==> le) f }
-; order := @Order_fun _ _ a.(order) b.(order) |}.
+{| T := PFun a b
+; order := @Order_fun a b |}.
 
 Definition Order_unit : Order unit.
 refine
@@ -62,11 +76,12 @@ Canonical Structure otype_unit : otype :=
 
 
 Definition otype_apply {a b : otype} (f : otype_fun a b) (x : a) : b :=
-  (projT1 f) x.
+  f.(function) x.
 
 Lemma Proper_otype_apply {a b : otype}
-  : Proper (@le _ (otype_fun a b).(order) ==> @le _ a.(order) ==> @le _ b.(order)) (@otype_apply a b).
+: Proper (ole ==> ole ==> ole) (@otype_apply a b).
   red. red. red. intros.
+  red in H. unfold le in H. unfold order in H. simpl in H.
   eapply H. assumption.
 Defined.
 
@@ -81,10 +96,10 @@ Require Import Coq.Lists.List.
 Fixpoint otype_tuple (ls : list otype) : otype :=
   match ls with
   | nil => otype_unit
-  | l :: ls => otype_pair l (otype_tuple ls)
+  | l :: ls => otype_prod l (otype_tuple ls)
   end.
 
-Definition InCtx (ls : list otype) (t : otype) : Type :=
+Definition InCtx (ls : list otype) (t : otype) : otype :=
   otype_fun (otype_tuple ls) t.
 
 Definition App_ctx {ls a b} (f : InCtx ls (otype_fun a b)) (x : InCtx ls a)
@@ -102,9 +117,7 @@ eapply otype_abs.
 instantiate (1 := fun _ => x). red. red. intros. eapply Refl_le.
 Defined.
 
-Definition ToCtx {a} (x : InCtx nil a) : a.
-apply x. compute. tauto.
-Defined.
+Definition ToCtx {a} (x : InCtx nil a) : a := x.(function) tt.
 
 Definition Abs_ctx {ls a b} (x : InCtx (a :: ls) b) : InCtx ls (otype_fun a b).
 eapply otype_abs.
@@ -113,31 +126,27 @@ Unshelve.
 Focus 2.
 intro. eapply x. constructor. apply X. apply ctx.
 Focus 2.
-simpl. red. red. intros. destruct x; simpl. eapply p. constructor.
-simpl. eassumption. eapply Refl_le.
-red. red. intros.
-red. red. red. red. red. intros.
-simpl. destruct x. apply p. constructor; auto.
+abstract (simpl; do 2 red; intros; destruct x; simpl; eapply Proper_function0; constructor;
+          [ eassumption | eapply Refl_le ]).
+abstract (do 2 red; unfold le; simpl; do 2 red; intros; simpl; destruct x; apply Proper_function0; constructor; auto).
 Defined.
+
 
 Definition tuple_hd {x xs} : otype_fun (otype_tuple (x :: xs)) x.
 exists (@fst _ _).
-red. red. simpl. tauto.
+abstract (do 2 red; fold otype_tuple; intros; red in H; unfold le in H; simpl in H; tauto).
 Defined.
 
 Definition tuple_tl {x xs} : otype_fun (otype_tuple (x :: xs)) (otype_tuple xs).
 exists (@snd _ _).
-red. red. simpl. tauto.
+abstract (do 2 red; fold otype_tuple; intros; red in H; unfold le in H; simpl in H; tauto).
 Defined.
 
 Definition otype_compose {a b c} : otype_fun a b -> otype_fun b c -> otype_fun a c.
 intros.
 red. simpl.
-exists (fun x => projT1 X0 (projT1 X x)).
-red. red. intros.
-eapply (projT2 X0).
-eapply (projT2 X).
-eassumption.
+exists (fun x => function X0 (function X x)).
+abstract (do 2 red; intros; eapply (Proper_function X0); eapply (Proper_function X); eassumption).
 Defined.
 
 Fixpoint Var_ctx {a} (n : nat) {ls} {struct n}
@@ -159,7 +168,7 @@ Fixpoint Var_ctx {a} (n : nat) {ls} {struct n}
   | nil , S _ => fun x : None = Some a => match x with eq_refl => tt end
   end.
 
-(** * A Deeply Embedded Langauge **)
+(** * A Deeply Embedded Language **)
 (**********************************)
 Require Import ExtLib.Data.Member.
 Section fo.
@@ -186,10 +195,94 @@ Fixpoint oexprD {ls} {ot} (e : oexpr ls ot) : InCtx ls ot :=
   match e in oexpr _ ot return InCtx ls ot with
   | Const _ t c => Lift_ctx c
   | Var v => let '(existT _ n pf) := member_to_nat v in Var_ctx n pf
-  | @App _ d c f x => 
+  | @App _ d c f x =>
     App_ctx (oexprD f) (oexprD x)
   | Abs body => Abs_ctx (oexprD body)
   end.
+
+Require Import ExtLib.Data.HList.
+
+Fixpoint arrs (ls : list otype) (d : otype) : otype :=
+  match ls with
+  | nil => d
+  | l :: ls => otype_fun l (arrs ls d)
+  end.
+Fixpoint apps {vs ls : list otype} {d : otype} (f : oexpr vs (arrs ls d)) (xs : hlist (oexpr vs) ls)
+: oexpr vs d.
+refine (
+  match xs in hlist _ ls
+        return oexpr vs (arrs ls d) -> oexpr vs d
+  with
+  | Hnil => fun f => f
+  | @Hcons _ _ l ls x xs => fun f => @apps vs ls _ (@App _ _ _ f x) xs
+  end f).
+Defined.
+
+(*
+Section tele.
+  Context {T : Type}.
+  Variable F : list T -> T -> Type.
+
+  Inductive tele : list T -> Type :=
+  | Tend : tele nil
+  | Tcons : forall t ts, F ts t -> tele ts -> tele (t :: ts).
+End tele.
+
+Section rem.
+  Context {T} {F : list T -> T -> Type}.
+  Fixpoint tele_rem  {ts} (t : tele (fun ts t => option (F ts t)) ts) : list T :=
+    match t with
+    | Tend _ => nil
+    | @Tcons _ _ t _ None ts => t :: tele_rem ts
+    | @Tcons _ _ _ _ (Some _) ts => tele_rem ts
+    end.
+End rem.
+*)
+
+Section Subst.
+  Context {T : Type}.
+  Variable F : list T -> T -> Type.
+  Inductive Subst : list T -> list T -> Type :=
+  | Snil : Subst nil nil
+  | Sterm : forall ts ts' t, F ts' t -> Subst ts ts' -> Subst (t :: ts) ts'
+  | Sskip : forall ts ts' t, Subst ts ts' -> Subst (t :: ts) (t :: ts').
+End Subst.
+
+(* NOTE: You can not implement this when you have a shallow encoding of types
+Fixpoint oexpr_red {ls' ls ds} {ot}
+         (g : Subst oexpr ls ls')
+         (e : oexpr ls (arrs ds ot))
+         (xs : hlist (oexpr ls') ds)
+: oexpr ls' ot.
+refine (
+  match e in oexpr _ ot'
+        return ot' = arrs ds ot -> oexpr ls' ot
+  with
+  | Const _ t c => fun pf =>
+                     _
+  | Var v => _
+  | @App _ d c f x => fun pf =>
+    @oexpr_red _ _ (d :: ds) ot g
+               match pf in _ = X return oexpr _ (otype_fun _ X) with
+               | eq_refl => f
+               end (Hcons (@oexpr_red _ _ nil d g x Hnil) xs)
+  | @Abs _ d c body =>
+    match xs in hlist _ ds
+          return otype_fun d c = arrs ds ot -> oexpr ls' ot
+    with
+    | Hnil => fun pf : otype_fun d c = ot =>
+      match pf with
+      | eq_refl => @Abs _ d c (@oexpr_red _ _ nil _ (@Sskip _ _ _ _ _ g)
+                                          body
+                                          Hnil)
+      end
+    | Hcons x xs => _
+    end
+  end eq_refl).
+Focus 3. simpl.
+refine
+  (fun pf => @oexpr_red ls' (_ :: ls) _ _ (Sterm _ x g) _ xs).
+*)
 
 Definition OExprD {ot} (e : oexpr nil ot) : ot :=
   ToCtx (oexprD e).
@@ -203,8 +296,9 @@ Arguments MN {_ _ _ _} _ : clear implicits.
 (* A very simple example *)
 Eval compute in OExprD (Abs (otype_eq nat) (Var MZ)).
 
-Definition otype_abs_eq {T} {a : otype} (F : T -> a) : otype_fun (otype_eq T) a.
-red. red. exists F. red. red. intros. compute in H. subst. eapply Refl_le.
+Definition otype_abs_eq {T} {a : otype} (F : T -> a)
+: otype_fun (otype_eq T) a.
+red. exists F. red. red. intros. compute in H. simpl in H. subst. eapply Refl_le.
 Defined.
 
 Definition inj {a:otype} (x : a) : a := x.
