theories/OMonad.v
@@ -1,0 +1,508 @@
+Require Import Coq.Setoids.Setoid.
+Require Import PredMonad.OrderedTerms.
+
+(***
+ *** The monad typeclass
+ ***)
+
+Notation "x '-o>' y" := (otype_fun x y) (right associativity, at level 99).
+Notation "x ~~ y" := (@oequiv _ x y) (no associativity, at level 70).
+Notation "x <~ y" := (@ole _ x y) (no associativity, at level 70).
+Notation "x @ y" := (otype_apply x y) (left associativity, at level 11, y at level 0).
+Notation "x $ y" := (otype_apply x y) (left associativity, at level 11, y at level 200, only parsing).
+
+Ltac make_cons T n :=
+  let rec go n :=
+      lazymatch n with
+      | 0 => uconstr:(@cons T _ _)
+      | S ?Z =>
+        let p := go Z in
+        uconstr:(@cons T _ p)
+      end
+  in
+  let z := go n in
+  refine z.
+
+
+Delimit Scope ctx_scope with ctx.
+
+Notation "x @ y" := (@App_ctx _ _ _ x%ctx y%ctx) (left associativity, at level 11, y at level 0) : ctx_scope.
+Notation "x $ y" := (@App_ctx _ _ _ x%ctx y%ctx) (left associativity, at level 11, y at level 200, only parsing) : ctx_scope.
+Notation "\ t => y" := (@Abs_ctx _ t _ y%ctx) (left associativity, at level 200) : ctx_scope.
+Notation "! x" := (@Lift_ctx _ _ x%ctx) (no associativity, at level 0) : ctx_scope.
+Notation "# n" := (@Var_ctx _ n%nat ltac:(make_cons otype n) eq_refl) (at level 0) : ctx_scope.
+Arguments ToCtx {_} _%ctx.
+Arguments Abs_ctx {_ _ _} _%ctx.
+Arguments App_ctx {_ _ _} (_ _)%ctx.
+
+
+Class OMonad (M : otype -> otype) : Type :=
+{ returnM : forall {A : otype}, A -o> (M A)
+; bindM : forall {A B : otype}, M A -o> (A -o> M B) -o> M B
+; monad_return_bind : forall (A B : otype) (x : A) (f : A -o> M B),
+    bindM @ (returnM @ x) @ f ~~ f @ x
+; monad_bind_return : forall A (m : M A),
+    bindM @ m @ returnM ~~ m
+; monad_assoc : forall {A B C : otype} m (f : A -o> M B) (g : B -o> M C),
+    bindM @ (bindM @ m @ f) @ g ~~
+    bindM @ m $ ToCtx (\ A => !bindM @ (!f @ #0) @ !g)
+}.
+
+
+Instance Reflexive_ole {T} : Reflexive (@ole T).
+Proof. red. intros. red. destruct T. eapply Refl_le. Qed.
+Instance Transitive_ole {T} : Transitive (@ole T).
+Proof. red. intros. red. destruct T. eapply Trans_le; eauto. Qed.
+
+Instance Reflexive_oequiv {T} : Reflexive (@oequiv T).
+Proof. red. intros. red. destruct T. split; eapply Refl_le. Qed.
+Instance Transitive_oequiv {T} : Transitive (@oequiv T).
+Proof. red. intros. red. destruct T. destruct H; destruct H0; split; etransitivity; eauto. Qed.
+
+
+Instance Proper_oequiv_iff {A : otype} : Morphisms.Proper (oequiv ==> oequiv ==> iff) (@oequiv A).
+Proof. Admitted.
+Instance Proper_oequiv_flip_impl {A : otype} : Morphisms.Proper (oequiv ==> oequiv ==> Basics.flip Basics.impl) (@oequiv A).
+Proof. Admitted.
+Instance Proper_oequiv_impl {A : otype} : Morphisms.Proper (oequiv ==> oequiv ==> Basics.impl) (@oequiv A).
+Proof. Admitted.
+Instance Proper_otype_apply {A B} : Morphisms.Proper (oequiv ==> oequiv ==> oequiv) (@otype_apply A B).
+Proof. Admitted.
+
+Typeclasses Opaque oequiv ole.
+
+
+(***
+ *** The Identity Monad
+ ***)
+
+Definition Identity (X:otype) := X.
+Instance OMonad_Identity : OMonad Identity :=
+{ returnM := fun A => ToCtx (\ A => #0)
+; bindM  := fun A B => ToCtx (\ Identity A => \ (A -o> Identity B) => #0 @ #1)
+}.
+Proof.
+{ reflexivity. }
+{ reflexivity. }
+{ reflexivity. }
+Qed.
+
+(** Pair Functions
+ **)
+Definition otype_pair {A B : otype} : A -o> B -o> otype_prod A B.
+  refine (ToCtx (\ _ => \ _ => _)).
+  red. simpl. exists (fun ba_ => (fst (snd ba_), fst ba_)).
+  abstract (do 2 red; split; simpl; apply H).
+Defined.
+
+Definition pair_fst {A B : otype} : otype_prod A B -o> A.
+  exists fst.
+  abstract (do 2 red; simpl; intros; apply H).
+Defined.
+
+Definition pair_snd {A B : otype} : otype_prod A B -o> B.
+  exists snd.
+  abstract (do 2 red; simpl; intros; apply H).
+Defined.
+
+Definition pair_elim {A B C : otype} : otype_prod A B -o> (A -o> B -o> C) -o> C :=
+  ToCtx (\ _ => \ _ => #0 @ (!pair_fst @ #1) @ (!pair_snd @ #1)).
+
+Lemma otype_ext_eq : forall {A B : otype} (f g : A -o> B),
+    (forall x, f @ x ~~ g @ x) ->
+    f ~~ g.
+Proof.
+  intros.
+  destruct f; destruct g; simpl in *.
+  split.
+  { red. simpl. red. intros.
+    etransitivity.
+    eapply Proper_function. eassumption.
+    eapply H. }
+  { red. simpl. red. intros.
+    etransitivity.
+    eapply Proper_function0. eassumption.
+    eapply H. }
+Qed.
+
+Opaque otype_apply.
+
+(** Tuple Reduction **)
+Lemma tuple_hd {A : otype} {As : list otype} x xs
+: @tuple_hd A As @ (otype_pair @ x @ xs) ~~ x.
+Proof. reflexivity. Defined.
+Lemma tuple_tl {A : otype} {As : list otype} x xs
+  : @tuple_tl A As @ (otype_pair @ x @ xs) ~~ xs.
+Proof. reflexivity. Defined.
+
+Lemma tuple_tl_pair {A : otype} {Bs : list otype} (x : A) (y : otype_tuple Bs)
+  : OrderedTerms.tuple_tl @ (x,y) ~~ y.
+Proof. reflexivity. Defined.
+Lemma tuple_hd_pair {A : otype} {Bs : list otype} (x : A) (y : otype_tuple Bs)
+  : OrderedTerms.tuple_hd @ (x,y) ~~ x.
+Proof. reflexivity. Defined.
+
+(** Generic Reduction **)
+Lemma otype_apply_ToCtx {B} (f : InCtx nil B)
+: ToCtx f ~~ f @ tt.
+Proof. reflexivity. Defined.
+Lemma otype_apply_Abs_ctx {A B G} (f : InCtx (A :: G) B) (x : A) gs
+: Abs_ctx f @ gs @ x ~~ f @ (x, gs).
+Proof. reflexivity. Defined.
+Lemma otype_apply_App_ctx {A B G} (f : InCtx G (A -o> B)) x gs
+: otype_apply (App_ctx f x) gs ~~ otype_apply (f @ gs) (x @ gs).
+Proof. reflexivity. Defined.
+Lemma otype_apply_Lift_ctx {A : otype} {G : list otype} (f : A) gs
+: otype_apply (Lift_ctx (ls:=G) f) gs ~~ f.
+Proof. reflexivity. Defined.
+Lemma otype_apply_Var_ctx_O {A : otype} {G : list otype} (x : A)
+      (xs : otype_tuple G)
+: otype_apply (Var_ctx (a:=A) (ls:=A::G) 0 eq_refl) (x, xs) ~~ x.
+Proof. reflexivity. Qed.
+(** NOTE: Most things here are immediate from reflexivity, however, we don't
+ ** want to compute them because we only want to reduce in these instances.
+ ** If we do unconstrained reduction, then we will expose proofs and everything
+ ** will slow down.
+ **)
+
+Lemma otype_apply_Var_ctx_S {A B : otype} {G : list otype} n pf (x : A)
+      (xs : otype_tuple G)
+  : otype_apply (Var_ctx (a:=B) (ls:=A::G) (S n) pf) (x, xs) ~~
+                otype_apply (Var_ctx n pf) xs.
+Proof. simpl. unfold otype_compose.
+       generalize (Var_ctx n pf). intros.
+       destruct t.
+       simpl. reflexivity.
+Qed.
+Lemma otype_abs_otype_apply : forall {A B : otype} f pf x,
+    (@otype_abs A B f pf @ x) ~~ f x.
+Proof. reflexivity. Qed.
+
+
+Instance Proper_App_ctx G A B
+  : Morphisms.Proper (oequiv ==> oequiv ==> oequiv) (@App_ctx G A B).
+Proof. Admitted.
+
+Instance Proper_Abs_ctx G B A : Morphisms.Proper (oequiv ==> oequiv) (@Abs_ctx G A B).
+Proof. Admitted.
+
+Lemma ToCtx_eq {B} (f : InCtx nil B)
+  : ToCtx f = f @ tt.
+Proof. reflexivity. Qed.
+
+Instance Symmetric_oequiv {A} : Symmetric (@oequiv A).
+Proof. red. unfold oequiv. tauto. Qed.
+
+Hint Rewrite @otype_apply_Abs_ctx @ToCtx_eq
+     @otype_apply_Abs_ctx @otype_apply_App_ctx
+     @otype_apply_Lift_ctx @otype_apply_Var_ctx_S @otype_apply_Var_ctx_O
+  : reduce.
+Hint Rewrite @otype_abs_otype_apply : reduce.
+
+Lemma pair_elim_red {A B C : otype} (f : A -> B -> C)  pf' pf x :
+  pair_elim @ x @ (@otype_abs _ _ (fun x => @otype_abs _ _ (f x) (pf' x)) pf)
+  ~~ f (pair_fst @ x) (pair_snd @ x).
+Proof. Admitted.
+Lemma pair_elim_pair_red {A B C : otype} (f : A -o> B -o> C) x y :
+  pair_elim @ (otype_pair @ x @ y) @ f ~~ f @ x @ y.
+Proof. Admitted.
+Lemma otype_compose_red {A B C : otype} (f : A -o> B) (g : C -o> A) (x : C) :
+  otype_compose g f @ x ~~ f $ g $ x.
+Proof. Admitted.
+
+Lemma otype_pair_eta_contract {A B} (x : otype_prod A B) :
+  otype_pair @ (pair_fst @ x) @ (pair_snd @ x) ~~ x.
+Proof. Admitted.
+Lemma pair_elim_arr {A B C : otype} x (f : A -o> B -o> C)
+  : pair_elim @ x @ f ~~ f @ (pair_fst @ x) @ (pair_snd @ x).
+Proof. Admitted.
+
+Hint Rewrite @pair_elim_pair_red @otype_pair_eta_contract : reduce_pair.
+Hint Rewrite @pair_elim_arr : reduce_pair.
+
+(** TODO: move this outward **)
+Arguments otype_abs {_ _} _ {_} : clear implicits.
+
+Existing Instance Reflexive_oequiv.
+
+Existing Instance Transitive_oequiv.
+
+
+(***
+ *** The State Monad
+ ***)
+Section with_state.
+  Context {s : otype}.
+
+  Definition State (x : otype) := s -o> otype_prod x s.
+  Instance OMonad_State : OMonad State :=
+  { returnM := fun A => ToCtx (\ A => \ s => !otype_pair @ #1 @ #0)
+  ; bindM   := fun A B => ToCtx (\ State A => \ (A -o> State B) => \ s =>
+                                 !pair_elim @ (#2 @ #0) @ #1)
+  }.
+  Proof.
+  { intros. eapply otype_ext_eq; intros.
+    autorewrite with reduce reduce_pair.
+    reflexivity. }
+  { intros.
+    repeat (eapply otype_ext_eq; intros).
+    rewrite_strat (bottomup (hints reduce)).
+    rewrite_strat (topdown @otype_apply_Abs_ctx).
+    autorewrite with reduce reduce_pair.
+    reflexivity. }
+  { intros.
+    repeat (eapply otype_ext_eq; intros).
+    autorewrite with reduce reduce_pair.
+    reflexivity. }
+  Qed.
+End with_state.
+
+Hint Rewrite @monad_return_bind @monad_bind_return
+     @monad_assoc : reduce_monad.
+
+Lemma otype_pair_fst_pair : forall {A B : otype} (x : A) (y : B),
+    (pair_fst $ otype_pair @ x @ y) ~~ x.
+Proof. reflexivity. Qed.
+Lemma otype_pair_snd_pair : forall {A B : otype} (x : A) (y : B),
+    (pair_snd $ otype_pair @ x @ y) ~~ y.
+Proof. reflexivity. Qed.
+Hint Rewrite @otype_pair_fst_pair @otype_pair_snd_pair : reduce_pair.
+
+
+Section StateT.
+  Variable s : otype.
+  Variable m : otype -> otype.
+  Variable Mm : OMonad m.
+
+  (** This is hack to get around a bug in rewriting *)
+  Ltac force_rewrite :=
+    match goal with
+    | |- context [ @otype_apply ?Ta ?Tb (@otype_apply (otype_tuple ?G) (otype_fun ?Ta ?Tb) (@Abs_ctx ?G _ _ ?A) ?B) ?C ] =>
+      generalize (@otype_apply_Abs_ctx Ta Tb G A C B) ;
+      match goal with
+      | |- (?X ~~ _) -> _ => generalize X
+      end;
+      let x := fresh in
+      intro x ;
+      let H := fresh in
+      let rw := repeat simple eapply Proper_otype_apply;
+                first [ eapply H | reflexivity ] in
+      intro H; (etransitivity;
+                [ rw
+                | first [ clear H ; clear x
+                        | etransitivity ; [ | symmetry; rw ] ] ])
+    end.
+
+  Instance Proper_Lift_ctx A G
+  : Morphisms.Proper (oequiv ==> oequiv) (@Lift_ctx A G).
+  Proof.
+    do 2 red. simpl. unfold Lift_ctx. intros.
+    eapply otype_ext_eq.
+    intros.
+    autorewrite with reduce. assumption.
+  Qed.
+
+  Fixpoint otype_tuple_concat {A B} {struct A}
+  : otype_tuple A -o> otype_tuple B -o> otype_tuple (A ++ B) :=
+    match A as A
+          return otype_tuple A -o> otype_tuple B -o> otype_tuple (A ++ B)
+    with
+    | nil => ToCtx (\ _ => \ _ => #0)
+    | List.cons a b => ToCtx (\ (otype_tuple (a :: b)) => \ otype_tuple B =>
+      !otype_pair @ (!OrderedTerms.tuple_hd @ #1)
+       @ (!otype_tuple_concat @ (!OrderedTerms.tuple_tl @ #1) @ #0))%ctx
+    end.
+
+  Definition Shifts_ctx {A B G} (f : InCtx (A ++ G) B) (g : otype_tuple G)
+  : InCtx A B.
+  red. simpl. econstructor.
+  Unshelve.
+  Focus 2. intro. eapply f.
+  eapply otype_tuple_concat; eassumption.
+  red. red. intros. red. eapply f.
+  eapply otype_tuple_concat; eauto. eapply Reflexive_ole.
+  Defined.
+
+(*
+  Definition Shift_ctx {A B G} (f : InCtx (A :: G) B) (g : otype_tuple G)
+    : InCtx (A :: nil) B := Shifts_ctx 
+    simpl in *. eexists (fun x_ => f.(function) (pair (pair_fst @ x_) g)).
+    simpl. red. red. intros.
+    eapply Proper_function. red. simpl. split.
+    apply H. reflexivity.
+  Defined.
+*)
+
+  Lemma otype_apply_Abs_ctx_shift {A B G} (f : InCtx (A :: G) B) gs
+  : otype_apply (Abs_ctx f) gs ~~ Abs_ctx (Shifts_ctx (A:=A::nil) f gs) @ tt.
+  Proof.
+    apply otype_ext_eq. intros.
+    reflexivity.
+  Qed.
+  Lemma Shift_ctx_App_ctx {A B : otype} {Z G : list otype}
+        (f : InCtx (Z ++ G) (A -o> B)) x g
+  : Shifts_ctx (App_ctx f x) g ~~ App_ctx (Shifts_ctx f g) (Shifts_ctx x g).
+  Proof.
+    eapply otype_ext_eq; intros.
+    reflexivity.
+  Qed.
+(*
+  Lemma Shift_ctx_Var_ctx_0 {A : otype} {G : list otype}
+        (pf : Some A = Some A) g
+    : Shift_ctx (A:=A) (G:=G) (Var_ctx (ls:=A::G) 0 pf) g ~~
+                (Var_ctx (ls:=A::nil) 0 pf).
+  Proof. Admitted.
+  Lemma Shift_ctx_Var_ctx_S {A B : otype} {G : list otype}
+        n (pf : List.nth_error G n = Some A) g
+    : Shift_ctx (A:=B) (G:=G) (Var_ctx (ls:=B::G) (S n) pf) g ~~
+                Lift_ctx ((Var_ctx n pf) @ g).
+  Proof. Admitted.
+  Lemma Shift_ctx_Lift_ctx {A B : otype} {G : list otype} (x : B) y
+    : Shift_ctx (A:=A) (G:=G) (Lift_ctx x) y ~~ Lift_ctx x.
+  Proof. Admitted.
+*)
+
+  Require Import Coq.Lists.List.
+(*
+  Lemma Shifts_ctx_Abs_ctx (A B C : otype) (G : list otype) (f : InCtx (C :: A :: G) B) (x : otype_tuple G)
+  : Shift_ctx (Abs_ctx f) x ~~ Abs_ctx (Shifts_ctx (A:=C::A::nil) (B:=B) (G:=G) f x).
+  Proof. Admitted.
+*)
+  Lemma Shifts_ctx_Abs_ctx (A : list otype) (B C : otype) (G : list otype) (f : InCtx (C :: A ++ G) B) (x : otype_tuple G)
+  : Shifts_ctx (A:=A) (Abs_ctx f) x ~~
+               Abs_ctx (Shifts_ctx (A:=C::A) (B:=B) (G:=G) f x).
+  Proof.
+    repeat (eapply otype_ext_eq; intros).
+    reflexivity.
+  Qed.
+  Lemma Shifts_ctx_App_ctx {A B : otype} {Z G : list otype}
+        (f : InCtx (Z ++ G) (A -o> B)) x g
+  : Shifts_ctx (App_ctx f x) g ~~ App_ctx (Shifts_ctx f g) (Shifts_ctx x g).
+  Proof.
+    repeat (eapply otype_ext_eq; intros).
+    reflexivity.
+  Qed.
+  Definition n_minus_0_is_n n : n - 0 = n :=
+    match n as n return n - 0 = n with
+    | 0 => eq_refl
+    | S n => eq_refl
+    end.
+
+  Fixpoint nth_error_pick_side {A} (xs ys : list otype) (n : nat)
+  : nth_error (xs ++ ys) n = Some A ->
+    {nth_error xs n = Some A} + {nth_error ys (n - length xs) = Some A} :=
+    match xs as xs
+          return nth_error (xs ++ ys) n = Some A ->
+                 {nth_error xs n = Some A} + {nth_error ys (n - length xs) = Some A}
+    with
+    | nil => fun pf => right match eq_sym (n_minus_0_is_n n) with
+                             | eq_refl => pf
+                             end
+    | x :: xs => match n as n
+                       return nth_error (x :: xs ++ ys) n = Some A ->
+                              {nth_error (x :: xs) n = Some A} + {nth_error ys (n - S (length xs)) = Some A}
+                 with
+                 | 0 => fun pf => left pf
+                 | S n => @nth_error_pick_side A xs ys n
+                 end
+    end.
+
+  Lemma Shifts_ctx_Var_ctx {A : otype} {Bs G : list otype}
+        n (pf : List.nth_error (Bs++G) n = Some A) g
+  : Shifts_ctx (A:=Bs) (G:=G) (Var_ctx (ls:=Bs++G) n pf) g ~~
+               match nth_error_pick_side Bs G n pf with
+               | left pf => @Var_ctx _ _ _ pf
+               | right pf => @Lift_ctx Bs A ((Var_ctx (n - List.length Bs) pf) @ g)
+               end.
+  Proof.
+    repeat (eapply otype_ext_eq; intros).
+    generalize dependent n.
+    induction Bs; simpl; intros.
+    { unfold Shifts_ctx. simpl.
+      Transparent otype_apply.
+      unfold otype_apply. simpl.
+      generalize (eq_sym (n_minus_0_is_n n)); intros.
+      generalize dependent (n-0).
+      intros; subst. reflexivity. }
+    { destruct n.
+      { simpl in *; clear.
+        admit. }
+      { admit. } }
+  Admitted.
+
+  Hint Rewrite @otype_apply_Abs_ctx_shift @Shift_ctx_App_ctx
+       @Shifts_ctx_Abs_ctx
+       @Shifts_ctx_App_ctx
+       @Shifts_ctx_Var_ctx
+    : reduce_shift.
+
+
+  Lemma Shifts_ctx_Lift_ctx {B : otype} {A G : list otype} (x : B) y
+    : Shifts_ctx (A:=A) (G:=G) (Lift_ctx x) y ~~ Lift_ctx x.
+  Proof. Admitted.
+  Instance Proper_pair {A B : otype} : Morphisms.Proper (oequiv ==> oequiv ==> oequiv) (@pair A B).
+  Proof. red. red. red. intros.
+         do 2 constructor; first [ apply H | apply H0 ].
+  Qed.
+
+  Lemma otype_apply_Var_ctx_O'
+    : forall (A : otype) (G : list otype) (x : A) (xs : otype_tuple G),
+      @oequiv A
+              (@otype_apply (otype_tuple (@cons otype A G)) A
+                            (@Var_ctx A O (@cons otype A G)
+                                      (@eq_refl (option otype) (@Some _ A)))
+                            (@pair A (otype_tuple G) x xs)) x.
+  Proof. Admitted.
+
+  Definition StateT (x : otype) : otype := s -o> m (otype_prod x s).
+  Instance OMonad_StateT : OMonad StateT :=
+  { returnM := fun A => ToCtx (\ A => \ s => !returnM $ !otype_pair @ #1 @ #0)
+  ; bindM   := fun A B => ToCtx (\ StateT A => \ (A -o> StateT B) => \ s =>
+                                 !bindM @ (#2 @ #0) @ \ (otype_prod A s) =>
+                                 !pair_elim @ #0 @ \ A => \ s =>
+                                   #4 @ #1 @ #0)
+  }.
+  Proof.
+  { intros.
+    repeat (eapply otype_ext_eq; intros).
+    repeat rewrite ToCtx_eq.
+    unfold StateT.
+    autorewrite with reduce reduce_pair reduce_monad.
+    reflexivity. }
+  { intros.
+    repeat (eapply otype_ext_eq; intros).
+    unfold StateT.
+    autorewrite with reduce reduce_pair reduce_monad.
+    etransitivity; [ | eapply monad_bind_return ].
+    eapply Proper_otype_apply; [ reflexivity | ].
+    repeat (eapply otype_ext_eq; intros).
+    autorewrite with reduce reduce_pair.
+    reflexivity. }
+  { intros.
+    repeat (eapply otype_ext_eq; intros).
+    rewrite ToCtx_eq.
+    rewrite_strat repeat progress (outermost @otype_apply_Abs_ctx).
+    progress rewrite_strat repeat progress (outermost (hints reduce)).
+    Ltac fwd :=
+      repeat first [ rewrite otype_apply_Abs_ctx
+                   | rewrite otype_apply_App_ctx
+                   | rewrite otype_apply_Lift_ctx
+                   | (progress repeat rewrite otype_apply_Var_ctx_S)
+                   | rewrite otype_apply_Var_ctx_O ].
+    fwd.
+    rewrite monad_assoc.
+    eapply Proper_otype_apply.
+    eapply Proper_otype_apply. reflexivity.
+    Ltac ext := repeat (eapply otype_ext_eq; intros).
+    reflexivity.
+    rewrite ToCtx_eq.
+    ext.
+    fwd.
+    do 2 rewrite pair_elim_arr.
+    fwd.
+    eapply Proper_otype_apply. reflexivity.
+    ext.
+    fwd.
+    reflexivity. }
+  Defined.
+End StateT.
